dw/Custom/List.v
@@ -1,8 +1,40 @@
-Require Export List.
+From Coq Require Export List.
 Export ListNotations.
 
-Definition null {A} (xs : list A) :=
-  match xs with
-  | nil => true
-  | _ => false
-  end.
+Definition replace_when {A : Type} (f : A -> bool) (new : A) (l : list A) :=
+  List.fold_right
+    (fun a tail => (if f a then new else a) :: tail)
+    [] l.
+
+Lemma filter_app: forall {A : Type} f (l1 l2 : list A),
+  filter f (l1 ++ l2) = filter f l1 ++ filter f l2.
+Proof.
+  induction l1; intros; trivial.
+  simpl.
+  destruct (f a); trivial.
+  simpl.
+  f_equal.
+  apply IHl1.
+Qed.
+
+Lemma filter_incl:
+  forall {A} (p : A -> bool) l, incl (filter p l) l.
+Proof.
+  unfold incl.
+  intros ? ? ? ? HIn.
+  rewrite filter_In in HIn.
+  destruct HIn; assumption.
+Qed.
+
+Lemma same_key_preserves_NoDup:
+  forall (T U : Type) (g : T -> U) (t t' : T) (prefix suffix : list T),
+    g t = g t' ->
+    NoDup (map g (prefix ++ t :: suffix)) ->
+    NoDup (map g (prefix ++ t' :: suffix)).
+Proof.
+  intros T U g t t' prefix suffix Heq HNoDup.
+  rewrite map_app in *.
+  simpl in *.
+  rewrite <- Heq.
+  trivial.
+Qed.
