dw/DeepWeb/Lib/SimpleSpec.v
@@ -1,0 +1,519 @@
+Generalizable Variable E.
+Typeclasses eauto := 6.
+
+From QuickChick Require Import QuickChick.
+
+Require Import Ascii.
+Require Import String.
+Require Import List.
+Require Import PArith.
+Require Fin.
+Import ListNotations.
+
+From Custom Require Import Show.
+
+Require Import DeepWeb.Free.Monad.Free.
+Import MonadNotations.
+Require Import DeepWeb.Free.Monad.Common.
+Import SumNotations.
+Import NonDeterminismBis.
+
+Require Import DeepWeb.Util.ByteType.
+
+Require Import DeepWeb.Lib.NetworkInterface.
+
+(* begin hide *)
+Set Warnings "-extraction-opaque-accessed,-extraction".
+Open Scope string_scope.
+(* end hide *)
+
+(* The observations that can be made by the spec.
+   This is parameterized by a type of "hints" that
+   can be used to help generating test cases. *)
+(* TODO: decide whether to restore hints. *)
+Inductive observerE : Type -> Type :=
+  (* Observe the creation of a new connection *)
+| ObsConnect : observerE connection_id
+
+  (* Observe a byte going into the server on a particular
+     connection *)
+| ObsToServer :
+    connection_id ->
+    observerE byte
+
+  (* Observe a byte going out of the server.
+     This action can return [None] "holes" as a way to hypothesize
+     that the server sent some message we haven't yet received,
+     so we can keep testing the rest of the trace.
+     We must be careful that, if a trace with holes is
+     rejected, then it must also be for any substitution
+     of actual values for those holes. *)
+| ObsFromServer :
+    connection_id -> observerE (option byte)
+.
+
+Definition obs_connect {E} `{observerE -< E} : M E connection_id :=
+  embed ObsConnect.
+
+Definition obs_to_server {E} `{observerE -< E} :
+  connection_id -> M E byte :=
+  embed ObsToServer.
+
+Definition obs_from_server {E} `{observerE -< E} :
+  connection_id -> M E (option byte) :=
+  embed ObsFromServer.
+
+(* Equality comparison, return a proof of equality of the
+   indices (this could be generalized to a complete decision
+   procedure). *)
+Definition observer_eq {X Y : Type}
+           (e1 : observerE X) (e2 : observerE Y) :
+  option (X = Y) :=
+  match e1, e2 with
+  | ObsConnect, ObsConnect => Some eq_refl
+  | ObsToServer c, ObsToServer c'
+  | ObsFromServer c, ObsFromServer c' =>
+    if c = c' ? then Some eq_refl else None
+  | _, _ => None
+  end.
+
+Definition coerce {X Y : Type} (p : X = Y) (x : X) : Y :=
+  match p in eq _ Y return Y with
+  | eq_refl => x
+  end.
+
+Definition specE := nondetE +' observerE.
+
+Definition itree_spec := M specE unit.
+
+(* Make an assertion on a value, if it exists. *)
+Definition assert_on {A}
+           (r : string) (oa : option A) (check : A -> bool) :
+  M specE unit :=
+  match oa with
+  | None => ret tt
+  | Some a =>
+    if check a then ret tt else fail ("assertion failed: " ++ r)
+  end.
+
+(* Helper for [obs_msg_to_server] *)
+CoFixpoint obs_msg_to_server'
+           (c : connection_id) (n : nat) (k : bytes -> M specE bytes) :
+  M specE bytes :=
+  match n with
+  | O => k ""
+  | S n =>
+    b <- ^ ObsToServer c;;
+    obs_msg_to_server' c n (fun bs => k (String b bs))
+  end.
+
+(* Observe a complete message sent to the server. *)
+Definition obs_msg_to_server (buffer_size : nat)
+           (c : connection_id) : M specE bytes :=
+  obs_msg_to_server' c buffer_size ret.
+
+(* Observe a complete message received from the server. *)
+CoFixpoint obs_msg_from_server
+           (c : connection_id) (msg : bytes) :
+  M specE unit :=
+  match msg with
+  | "" => ret tt
+  | String b0 msg =>
+    ob <- ^ ObsFromServer c;;
+    assert_on "bytes must match" ob (fun b1 => b1 = b0 ?);;
+    obs_msg_from_server c msg
+  end.
+
+(* The spec can be viewed as a set of traces. *)
+
+(* An [event] is an observer action together with its result. *)
+Inductive event :=
+| Event : forall X, observerE X -> X -> event.
+
+Arguments Event {X}.
+
+Definition show_event (ev : event) :=
+  match ev with
+  | Event _ e x =>
+    match e in observerE X return X -> _ with
+    | ObsConnect => fun c => show c ++ " !"
+    | ObsToServer c => fun b =>
+      show c ++ " <-- """ ++ pretty_char b ++ """"
+    | ObsFromServer c => fun ob =>
+      show c ++ " --> " ++
+        match ob with
+        | None => "?"
+        | Some b => """" ++ pretty_char b ++ """"
+        end
+    end x
+  end.
+
+Instance Show_event : Show event :=
+  { show := show_event }.
+
+Definition trace := list event.
+
+Definition match_obs {X Y R S : Type}
+           (e0 : observerE X)
+           (e1 : observerE Y)
+           (cont : S -> R)
+           (fail_ : R) :
+  X -> (Y -> S) -> R :=
+  match e0 in observerE X, e1 in observerE Y
+        return X -> (Y -> _) -> _ with
+  | ObsConnect, ObsConnect => fun x k => cont (k x)
+  | ObsToServer c, ObsToServer c' => fun x k =>
+    if c = c' ? then
+      cont (k x)
+    else
+      fail_
+  | ObsFromServer c, ObsFromServer c' => fun x k =>
+    if c = c' ? then
+      cont (k x)
+    else
+      fail_
+  | _, _ => fun _ _ => fail_
+  end.
+
+(* [exists x, k x = true] *)
+Definition nondet_exists {X : Type}
+           (e : nondetE X) (k : X -> bool) : bool :=
+  match e in nondetE X' return (X' -> X) -> _ with
+  | Or n _ =>
+    (fix go n0 : (Fin.t n0 -> X) -> bool :=
+       match n0 with
+       | O => fun _ => false
+       | S n0 => fun f => k (f Fin.F1) || go n0 (fun m => f (Fin.FS m))
+       end) n
+  end%bool (fun x => x).
+
+(* Basically, a trace [t] belongs to a tree if there is a path
+   through the tree (a list of [E0] effects) such that its
+   restriction to [observerE] events is [t].
+   Because trees are coinductive (in particular, they can contain
+   arbitrary sequences of [Tau] or [Vis] with invisible effects),
+   it is not possible to decide whether a trace matches the tree.
+   Thus we add a [fuel] parameter assumed to be "big enough"
+   for the result to be reliable. *)
+Fixpoint is_trace_of (fuel : nat) (s : itree_spec) (t : trace) : bool :=
+  match fuel with
+  | O => false
+  | S fuel =>
+    match s, t with
+    | Tau s, t => is_trace_of fuel s t
+    | Ret tt, [] => true
+    | Ret tt, _ :: _ => false
+    | Vis _ (| e1 ) k, Event _ e0 x :: t =>
+      match_obs e0 e1 (fun s => is_trace_of fuel s t)
+                false x k
+    | Vis _ (| e1 ) k, [] => true
+    (* The trace belongs to the tree [s] *)
+    | Vis _ ( _Or |) k, t =>
+      nondet_exists _Or (fun b => is_trace_of fuel (k b) t)
+    end
+  end.
+
+
+(* The traces produced by the tree [swap_spec] are very structured,
+   with sequences of bytes sent and received alternating tidily.
+   However, in general:
+   - the network may reorder some messages, so the traces
+     we actually see during testing will not be directly
+     checkable using [is_trace_of], they must be descrambled
+     first;
+   - a server implementation may also want to reorder responses
+     differently for performance and other practical reasons;
+     here we will consider a server correct if it cannot be
+     distinguished over the network from a server that actually
+     produces the same traces as the spec above.
+ *)
+
+(* The constraints on the network are:
+   - a connection must be open before bytes can be exchanged on it;
+   - two bytes going in the same direction on the same connection
+     must arrive in-order;
+   - if we get a byte [b1] from the server before we send some [b2]
+     to it, then the server definitely sent [b1] before it
+     can receive [b2]. ([FromServer,ToServer] cannot be descrambled
+     to [ToServer,FromServer], regardless of the connections
+     where the two events happen.)
+ *)
+
+(* Unary tree node carrying some event. *)
+Inductive eventE : Type -> Type :=
+| Happened : event -> eventE unit.
+
+(* We enumerate descramblings in a tree structure, using
+   [nondetE] to branch, so that each successful pat (i.e., not
+   leading to failure) is a descrambling of a given trace. *)
+Definition eventE' := nondetE +' eventE.
+
+(* Helper for [pick_event]. *)
+CoFixpoint pick_event' (t_prev t : trace) :
+  M eventE' trace :=
+  match t with
+  | [] => fail "empty trace"
+  | Event _ e _ as ev :: t =>
+    let pick_this :=
+        _ <- ^ Happened ev;;
+       ret (List.rev t_prev ++ t)%list in
+    disj "pick_event'"
+      ( match e with
+        | ObsConnect =>
+          if forallb (fun ev =>
+                match ev with
+                | Event _ (ObsFromServer _) _ => false
+                | _ => true
+                end) t_prev then
+            pick_this
+          else
+            fail "inaccessible ObsConnect"
+
+        | ObsToServer c =>
+          if forallb (fun ev =>
+               match ev with
+               | Event _ (ObsFromServer c') _ => false
+               | Event _ ObsConnect c'
+               | Event _ (ObsToServer c') _ => c <> c' ?
+               end) t_prev then
+            pick_this
+          else
+            fail "inaccessible ObsToServer"
+
+        | ObsFromServer c =>
+          if forallb (fun ev =>
+               match ev with
+               | Event _ (ObsToServer _) _ => true
+               | Event _ ObsConnect c'
+               | Event _ (ObsFromServer c') _ => c <> c' ?
+               end) t_prev then
+            pick_this
+          else
+            fail "inaccessible ObsFromServer"
+
+        end
+      | pick_event' (ev :: t_prev) t
+      )
+  end.
+
+(* Given a scrambled trace, remove one event that could potentially
+   be the next one in a descrambling.
+ *)
+Definition pick_event : trace -> M eventE' trace :=
+  pick_event' [].
+
+Definition is_ObsFromServer (ev : event) :=
+  match ev with
+  | Event _ (ObsFromServer _) _ => true
+  | _ => false
+  end.
+
+(* Once the only things left are messages sent to the server,
+   we drop them, since there is no response to compare them
+   against. *)
+CoFixpoint descramble (t : trace) : M eventE' unit :=
+  match filter is_ObsFromServer t with
+  | [] => ret tt
+  | _ :: _ =>
+    t' <- pick_event t;;
+    descramble t'
+  end.
+
+(* Functions to list the descrambled traces *)
+Section ListDescramble.
+
+Fixpoint list_eventE' (fuel : nat) (s : M eventE' unit)
+           (acc : list trace) (new : trace -> trace) :
+  option (list trace) :=
+  match fuel with
+  | O => None
+  | S fuel =>
+    match s with
+    | Tau s => list_eventE' fuel s acc new
+    | Ret tt => Some (new [] :: acc)
+    | Vis _ (| e ) k =>
+      match e in eventE X return (X -> _) -> _ with
+      | Happened ev => fun k =>
+        list_eventE' fuel (k tt) acc (fun t => new (ev :: t))
+      end k
+    | Vis X ( _Or |) k =>
+      match _Or in nondetE X' return (X' -> _) -> _ with
+      | Or n _ =>
+        (fix go n0 : (Fin.t n0 -> X) -> _ :=
+           match n0 with
+           | O => fun _ => Some acc
+           | S n0 => fun f =>
+             match list_eventE' fuel (k (f Fin.F1)) acc new with
+             | None => None
+             | Some acc => go n0 (fun m => f (Fin.FS m))
+             end
+           end) n
+      end (fun x => x)
+    end
+  end.
+
+(* [None] if not enough fuel. *)
+Definition list_eventE (fuel : nat) (s : M eventE' unit) :
+  option (list trace) :=
+  list_eventE' fuel s [] (fun t => t).
+
+(* Fuel of the order of [length t ^ 2] should suffice. *)
+Definition list_descramblings (fuel : nat) (t : trace) :
+  option (list trace) :=
+  list_eventE fuel (descramble t).
+
+(*
+Compute list_descramblings 50 [
+  Event ObsConnect 0;
+  Event (ObsToServer 0 tt) "A";
+  Event ObsConnect 1;
+  Event (ObsToServer 0 tt) "B";
+  Event (ObsFromServer 0) (Some "C")
+]%char.
+*)
+
+End ListDescramble.
+
+(* Those descramblings are still missing [ObsFromServer] events
+   with holes (i.e., with [None] in the last field of [Event]).
+   We will insert them as needed when comparing the tree of
+   descramblings with the spec tree. *)
+
+CoFixpoint select_event' {X}
+           (e : observerE X) (t_prev t : trace) :
+  M (nondetE +' eventE) (X * trace) :=
+  match t with
+  | [] =>
+    match e with
+    | ObsFromServer _ as e =>
+      (* If we're expecting a reply from the server, we
+         can temporarily put a hole to see what should happen
+         next. *)
+      ^ Happened (Event e None);;
+      ret (None, rev t_prev)
+    | _ => fail "no event left to pick"
+    end
+  | Event X' e' x as ev :: t =>
+    match observer_eq e' e with
+    | Some p => (* e' = e *)
+        ^ Happened ev;;
+        ret (coerce p x, rev t_prev ++ t)%list
+    | None => (* e' <> e *)
+      let try_next := Tau (select_event' e (ev :: t_prev) t) in
+      match e, e' with
+
+      | ObsConnect as e, ObsToServer _
+      | ObsToServer _ as e, (ObsConnect | ObsToServer _)
+      | ObsFromServer _ as e, _ =>
+        try_next
+
+        (* We're looking for a [Connect/ToServer] event
+           but there is still a [FromServer] event to explain. *)
+      | (ObsConnect | ObsToServer _), ObsFromServer _ =>
+        fail "inaccessible event"
+
+      | ObsConnect, ObsConnect => fail "should not happen"
+      end
+    end
+  end.
+
+Definition select_event {X} (e : observerE X) :
+  trace -> M (nondetE +' eventE) (X * trace) := select_event' e [].
+
+(* [s]: tree of acceptable traces (spec)
+   [t]: scrambled trace
+
+   The result tree has a [Ret] leaf iff there is a descrambled
+   trace accepted by [s] ([is_trace_of]).
+ *)
+CoFixpoint intersect_trace
+            (s : M (nondetE +' observerE) unit)
+            (t : trace) :
+  M (nondetE +' eventE) unit :=
+  match s with
+  | Tau s => Tau (intersect_trace s t)
+  | Ret tt =>
+    match filter is_ObsFromServer t with
+    | [] => ret tt
+    | _ :: _ => fail "unexplained events remain"
+    end
+  | Vis _ ( e |) k => Vis ( e |) (fun x => intersect_trace (k x) t)
+  | Vis X (| e ) k =>
+    match filter is_ObsFromServer t with
+    | [] => ret tt
+    | _ :: _ =>
+      xt <- select_event e t;;
+      let '(x, t) := xt in
+      intersect_trace (k x) t
+    end
+  end.
+
+CoFixpoint find' (ts : list (M (nondetE +' eventE) unit)) :
+  M emptyE bool :=
+  match ts with
+  | [] => ret false
+  | t :: ts =>
+    match t with
+    | Tau t => Tau (find' (t :: ts))
+    | Ret tt => ret true
+    | Vis X e k =>
+      match e with
+      | (| ev ) =>
+        match ev in eventE X' return (X' -> X) -> _ with
+        | Happened _ => fun id => Tau (find' (k (id tt) :: ts))
+        end (fun x => x)
+      | ( _Or |) =>
+        match _Or in nondetE X' return (X' -> X) -> _ with
+        | Or n _ => fun id =>
+          Tau (find' (map (fun n => k (id n)) every_fin ++ ts)%list)
+        end (fun x => x)
+      end
+    end
+  end.
+
+Inductive result := Found | NotFound | OutOfFuel.
+
+Definition option_to_list {A} (o : option A) : list A :=
+  match o with
+  | None => []
+  | Some a => [a]
+  end.
+
+Fixpoint to_result (fuel : nat) (m : M emptyE bool) : result :=
+  match fuel with
+  | O => OutOfFuel
+  | S fuel =>
+    match m with
+    | Ret b => if b then Found else NotFound
+    | Tau m => to_result fuel m
+    | Vis X e k => match e in emptyE X' with end
+    end
+  end.
+
+Definition is_scrambled_trace_of
+           (fuel : nat) (s : itree_spec) (t : trace) : result :=
+  to_result fuel (find' [intersect_trace s t]).
+
+Module EventNotations.
+
+Delimit Scope event_scope with event.
+
+(* Connection [c] is open. *)
+Notation "c !" := (Event ObsConnect c)
+(at level 30) : event_scope.
+
+(* Byte [b] goes to the server on connection [c]. *)
+Notation "c <-- b" := (Event (ObsToServer c) b%char)
+(at level 30) : event_scope.
+
+(* Byte [b] goes out of the server on connection [c]. *)
+Notation "c --> b" := (Event (ObsFromServer c) (Some b%char))
+(at level 30) : event_scope.
+
+(* Unknown byte goes out of the server on connection [c]. *)
+Notation "c --> ?" := (Event (ObsFromServer c) None)
+(at level 30) : event_scope.
+
+Open Scope event_scope.
+
+End EventNotations.
