dw/DeepWeb/Spec/ServerDefs.v
@@ -1,7 +1,9 @@
 Require Import Coq.ZArith.ZArith.
-From Custom Require Decidability.
-
 Open Scope Z.
 
+From Custom Require Import String.
+
 Definition BUFFER_SIZE : Z := 1024.
-Definition SERVER_PORT : Z := 80.
+Definition SERVER_PORT : Z := 8000.
+
+Definition INIT_MSG := repeat_string "0"%char (Z.to_nat BUFFER_SIZE).
