dw/DeepWeb/Spec/SingleSwapSequential_Impl.v
@@ -1,0 +1,36 @@
+Generalizable Variable E.
+
+From DeepWeb.Free.Monad
+     Require Import Free Common Verif.
+
+From QuickChick Require Import Decidability.
+
+From Custom Require Import List.
+Import ListNotations.
+
+Require Import DeepWeb.Spec.ServerDefs.
+Require Import DeepWeb.Lib.Socket.
+Require Import DeepWeb.Lib.TestDefaults.
+Require Import DeepWeb.Util.ByteType.
+
+Require Import String.
+
+Import SocketAPI.
+
+From Custom Require Monad.
+Import MonadNotations.
+
+CoFixpoint server_
+           (endpoint : endpoint_id)
+           (buffer_size : nat)
+           (last_msg : bytes) : M _ unit :=
+  c <- accept endpoint;;
+  msg <- recv_full c buffer_size;;
+  send c last_msg;;
+  server_ endpoint buffer_size msg.
+
+Definition server :=
+  server_
+    default_endpoint
+    default_buffer_size
+    default_init_message.
