dw/DeepWeb/Spec/SingleSwap_SimpleSpec.v
@@ -1,0 +1,166 @@
+Generalizable Variable E.
+Typeclasses eauto := 6.
+
+From QuickChick Require Import QuickChick.
+
+Require Import Ascii.
+Require Import String.
+Require Import List.
+Require Import PArith.
+Require Fin.
+Import ListNotations.
+
+From Custom Require Import
+     String.
+
+Require Import DeepWeb.Free.Monad.Free.
+Import MonadNotations.
+Require Import DeepWeb.Free.Monad.Common.
+Import SumNotations.
+Import NonDeterminismBis.
+
+Require Import DeepWeb.Util.ByteType.
+
+Require Import DeepWeb.Lib.NetworkInterface.
+Require Import DeepWeb.Lib.SimpleSpec.
+
+(* begin hide *)
+Set Warnings "-extraction-opaque-accessed,-extraction".
+Open Scope string_scope.
+(* end hide *)
+
+(* [conns]: open connections, used for generating test cases.
+   [last_msg]: last message received.
+ *)
+CoFixpoint swap_spec_loop
+           (buffer_size : nat)
+           (conns : list connection_id)
+           (last_msg : bytes) :
+  itree_spec :=
+  (* Accept a new connection. *)
+  c <- ^ ObsConnect;;
+  (* Exchange one pair of messages. *)
+  msg <- obs_msg_to_server buffer_size c;;
+  obs_msg_from_server c last_msg;;
+  swap_spec_loop buffer_size conns msg.
+
+Definition init_msg (buffer_size : nat) :=
+  repeat_string "0"%char buffer_size.
+
+Definition swap_spec_ buffer_size :=
+  swap_spec_loop buffer_size [] (init_msg buffer_size).
+
+Definition swap_spec_def := swap_spec_ 3.
+
+Section ExampleTraces.
+
+Import EventNotations.
+
+Example trace_example :
+  true = is_trace_of 100 swap_spec_def [
+    0 !;
+    0 <-- "a";
+    0 <-- "b";
+    0 <-- "c";
+    0 --> "0";
+    0 --> "0";
+    0 --> "0";
+    1 !;
+    1 <-- "d";
+    1 <-- "e";
+    1 <-- "f";
+    1 --> "a";
+    1 --> "b";
+    1 --> "c"
+  ].
+Proof. reflexivity. Qed.
+
+Example trace_example2 :
+  false = is_trace_of 100 swap_spec_def [
+    0 !;
+    0 <-- "a";
+    0 <-- "b";
+    0 <-- "c";
+    0 --> "1"
+    (* error: Initial state is 000 *)
+  ].
+Proof. reflexivity. Qed.
+
+Example scrambled_trace_example :
+  Found = is_scrambled_trace_of 1000 swap_spec_def [
+    0 !;
+    1 !;
+    0 <-- "a";
+    0 <-- "b";
+    0 <-- "c";
+    0 --> "0";
+    0 --> "0";
+    0 --> "0";
+    1 <-- "d";
+    1 <-- "e";
+    1 <-- "f";
+    1 --> "a";
+    1 --> "b";
+    1 --> "c"
+  ].
+Proof. reflexivity. Qed.
+
+Example scrambled_trace_example_2 :
+  Found = is_scrambled_trace_of 1000 swap_spec_def [
+    0 !;
+    1 !;
+    0 <-- "a";
+    0 <-- "b";
+    0 <-- "c";
+    1 <-- "d";
+    1 <-- "e";
+    1 <-- "f";
+    1 --> "a";
+    1 --> "b";
+    1 --> "c";
+    0 --> "0";
+    0 --> "0";
+    0 --> "0"
+  ].
+Proof. reflexivity. Qed.
+
+Example scrambled_trace_example_3 :
+  NotFound = is_scrambled_trace_of 1000 swap_spec_def [
+    0 !;
+    1 !;
+    0 <-- "a";
+    0 <-- "b";
+    0 <-- "c";
+    1 <-- "d";
+    1 <-- "e";
+    1 <-- "f";
+    0 --> "d";
+    0 --> "e";
+    0 --> "f"
+  ].
+Proof. reflexivity. Qed.
+
+Example bad_scrambled_trace_example :
+  NotFound = is_scrambled_trace_of 1000 swap_spec_def [
+    0 !;
+    1 !;
+    2 !;
+    0 <-- "a";
+    0 <-- "b";
+    0 <-- "c";
+    1 <-- "d";
+    1 <-- "e";
+    1 <-- "f";
+    2 <-- "g";
+    2 <-- "h";
+    2 <-- "i";
+    1 --> "g";
+    1 --> "h";
+    1 --> "i";
+    2 --> "d";
+    2 --> "e";
+    2 --> "f"
+  ].
+Proof. reflexivity. Qed.
+
+End ExampleTraces.
