dw/DeepWeb/Test/Client.v
@@ -1,0 +1,44 @@
+From Coq Require Import
+     Extraction
+     String.
+From DeepWeb Require Import ByteType.
+
+(* begin hide *)
+Set Warnings "-extraction-opaque-accessed,-extraction".
+(* end hide *)
+
+Parameter file_descr : Type.
+
+Parameter close  : file_descr -> unit.
+Parameter init   : forall {A}, A -> A.
+Parameter recvb  : file_descr -> option byte.
+Parameter sendb  : file_descr -> byte -> unit.
+Parameter socket : unit -> file_descr.
+
+Extract Constant file_descr => "Unix.file_descr".
+
+Extract Constant close  => "fun sock ->
+  Unix.shutdown sock Unix.SHUTDOWN_ALL".
+Extract Constant init => "fun x ->
+  ignore (Unix.system ""make server"");
+  Unix.sleep 1;
+  x".
+Extract Constant recvb  => "fun sock ->
+  let bs = Bytes.create 1 in
+  match Unix.recv sock bs 0 1 [] with
+  | exception Unix.Unix_error(Unix.EAGAIN, _, _) ->
+     None
+  | 0 -> None
+  | k ->
+     if k = 1 then
+       Some (Bytes.get bs 0)
+     else
+       None".
+Extract Constant sendb  => "fun sock c ->
+  ignore (Unix.send sock (Bytes.make 1 c) 0 1)".
+Extract Constant socket => "fun _ ->
+  let open Unix in
+  let sock = socket PF_INET SOCK_STREAM 0 in
+  connect sock (ADDR_INET (inet_addr_loopback, 8000));
+  setsockopt_float sock SO_RCVTIMEO 0.;
+  sock".
