dw/DeepWeb/Test/ExternalTest.v
@@ -1,0 +1,99 @@
+From Coq Require Import Basics List ZArith.
+From ExtLib Require Import Functor OptionMonad StateMonad.
+From QuickChick Require Import QuickChick.
+From DeepWeb Require Import
+     ByteType
+     Client
+     NetworkInterface
+     Rand
+     SimpleSpec.
+
+Import FunctorNotation ListNotations MonadNotation.
+Open Scope program_scope.
+
+Fixpoint filterSome {A} (l : list (option A)) : list A :=
+  match l with
+  | [] => []
+  | Some a :: l => a :: filterSome l
+  | None :: l => filterSome l
+  end.
+
+Definition recv_external (cid_fd : connection_id * file_descr) : option event :=
+  let (cid, fd) := cid_fd in
+  Event (ObsFromServer cid) ∘ Some <$> recvb fd.
+
+Definition Client := state (list (connection_id * file_descr)).
+
+Definition newConnection : Client (connection_id * file_descr) :=
+  connections <- get;;
+  let c := (length connections, socket tt) in
+  put (c::connections);;
+  ret c.
+
+Definition sendMessage (b : byte) : Client event :=
+  connections <- get;;
+  match connections with
+  | [] => c <- newConnection;;
+         ret (sendb (snd c) b);;
+         ret (Event (ObsToServer (fst c)) b)
+  | c0::_ =>
+    let c := nth (rand (length connections)) connections c0 in
+    ret (sendb (snd c) b);;
+    ret (Event (ObsToServer (fst c)) b)
+  end.
+
+Definition recvMessage (l : list (connection_id * file_descr)) : trace :=
+  filterSome (map recv_external l).
+
+Definition closeAll : Client (list unit) :=
+  connections <- get;;
+  put [];;
+  ret (map (close ∘ snd) connections).
+
+Fixpoint execute' (fuel : nat) (msgs : list byte) : Client trace :=
+  match fuel with
+  | 0 => closeAll;;
+        ret []
+  | S fuel =>
+    match msgs with
+    | [] =>
+      tr <- recvMessage <$> get;;
+      closeAll;;
+      ret tr
+    | msg::msgs' =>
+      if flip tt
+      then
+        ev <- sendMessage msg;;
+        evs <- execute' fuel msgs';;
+        ret (ev::evs)
+      else
+        if flip tt
+        then
+          connections <- get;;
+          evs <- execute' fuel msgs;;
+          ret ((recvMessage connections) ++ evs)
+        else
+          newConnection;;
+          execute' fuel msgs
+    end
+  end.
+
+Definition execute (msgs : list byte) : Client trace :=
+  init <$> execute' (length msgs * 3) msgs.
+
+Instance Checkable_result : Checkable result :=
+  {| checker r :=
+       match r with
+       | Found => checker true
+       | NotFound => checker false
+       | OutOfFuel => checker tt
+       end |}.
+
+Require Swap_SimpleSpec.
+
+Definition execute_prop (msgs : list byte) : Checker :=
+  let tr := evalState (execute msgs) [] in
+  whenFail (show tr)
+  (is_scrambled_trace_of 1000 (Swap_SimpleSpec.swap_spec_def) tr).
+
+(*! QuickChick execute_prop. *)
