dw/DeepWeb/Test/Rand.v
@@ -1,0 +1,7 @@
+From Coq Require Extraction.
+
+Parameter flip : unit -> bool.
+Parameter rand : nat -> nat.
+
+Extract Constant flip => "Random.bool".
+Extract Constant rand => "Random.int".
