dw/DeepWeb/Test/TestCLikeSpec.v
@@ -1,0 +1,64 @@
+(* Simulate a server, nondeterministically returning
+   the new state of the network. *)
+
+Typeclasses eauto := 6.
+
+From QuickChick Require Import QuickChick.
+From ExtLib Require Monad.
+
+Require Import Ascii.
+Require Import String.
+Require Import List.
+Require Import PArith.
+Require Fin.
+Import ListNotations.
+
+Require Import DeepWeb.Free.Monad.Free.
+Import MonadNotations.
+Require Import DeepWeb.Free.Monad.Common.
+Import SumNotations.
+Import NonDeterminismBis.
+Require Import DeepWeb.Free.Monad.Spec.
+
+Require Import DeepWeb.Lib.TestDefaults.
+Require Import DeepWeb.Util.ByteType.
+
+From DeepWeb Require Import
+     Lib.NetworkInterface
+     Lib.SimpleSpec
+     Lib.SimpleSpecTest.
+
+From DeepWeb.Spec Require
+     Swap_CLikeSpec
+     Swap_SimpleSpec.
+
+(* Enumerate the traces of the [server'] itree (swap server). *)
+Definition random_trace_server :=
+  random_trace 500 10 Swap_CLikeSpec.test_server.
+
+(*
+Sample random_trace_server.
+*)
+
+Definition test :=
+  check_trace_incl_def
+    Swap_SimpleSpec.swap_spec_def
+    Swap_CLikeSpec.test_server.
+
+(* Takes a few seconds *)
+(*! QuickChick test. *)
+
+Require Import DeepWeb.Spec.SingleSwap_SimpleSpec.
+Require Import DeepWeb.Spec.SingleSwapSequential_Impl.
+
+Module SingleSwap.
+
+Definition spec := swap_spec_ default_buffer_size.
+Definition impl := server.
+
+Definition test :=
+  check_trace_incl_def spec impl.
+
+End SingleSwap.
+
+(*! QuickChick SingleSwap.test. *)
